Auxiliary/AuxRulesEquivProofsScript.sml
@@ -5,15 +5,44 @@ open preamble
      AuxRulesSpecTheory
      AuxRulesIMPTheory
      ratTheory
-                                    
-  
+                                       
+   
 val _ = new_theory "AuxRulesEquivProofs"
-       
-val Logical_ElimAux_to_Functional = Q.store_thm ("Logical_ElimAux_to_Functional",
- `!st qu l c t p np bl2 nbl2 e h nh.
-        ELIM_CAND_Auxiliary c (qu,st,l) t p np bl2 nbl2 e h nh ==> (ELIM_CAND_Auxiliary_dec c (qu,st,l) t p np  bl2 nbl2 e h nh)`,
+
+val EWIN_Auxiliary_thm = Q.store_thm("EWIN_Auxiliary_thm",
+  `EWIN_Auxiliary_dec = EWIN_Auxiliary`,
+  simp[FUN_EQ_THM]  
+  \\ qx_gen_tac`params`  
+  \\ PairCases_on`params`  
+  \\ Cases 
+   >- (Cases    
+     >- rw[EWIN_Auxiliary_def,EWIN_Auxiliary_dec_def]   
+     >- (PairCases_on`p`  
+       \\ rw[EWIN_Auxiliary_def,EWIN_Auxiliary_dec_def]  
+       \\ metis_tac[NULL,NULL_EQ])) 
+   >- (Cases
+    >- rw[EWIN_Auxiliary_dec_def,EWIN_Auxiliary_def]
+    >- rw[EWIN_Auxiliary_dec_def,EWIN_Auxiliary_def]));   
  
-   REPEAT STRIP_TAC >> fs[ELIM_CAND_Auxiliary_def,ELIM_CAND_Auxiliary_dec_def]  
+ 
+val HWIN_Auxiliary_thm = Q.store_thm("HWIN_Auxiliary_thm",
+  `HWIN_Auxiliary_dec = HWIN_Auxiliary`,
+
+  simp[FUN_EQ_THM]
+  \\ qx_gen_tac`params`
+  \\ PairCases_on`params`
+  \\ Cases \\ Cases \\ rw[HWIN_Auxiliary_def,HWIN_Auxiliary_dec_def]
+  \\ PairCases_on`p`
+  \\ FULL_SIMP_TAC list_ss [HWIN_Auxiliary_def,HWIN_Auxiliary_dec_def,LENGTH_APPEND,NULL,NULL_EQ]
+  \\ rw[HWIN_Auxiliary_def,HWIN_Auxiliary_dec_def]
+  \\ rw[HWIN_Auxiliary_def,HWIN_Auxiliary_dec_def]);
+ 
+  
+val Logical_ElimAux_to_Functional = Q.store_thm ("Logical_ElimAux_to_Functional",
+ `!st qu l c ba t nt p np bl nbl bl2  e ne h nh.
+        ELIM_CAND_Auxiliary c (qu,st,l) ba t nt p np bl nbl bl2 e ne h nh ==> (ELIM_CAND_Auxiliary_dec c (qu,st,l) ba t nt p np bl nbl bl2 e ne h nh)`,
+  
+   REPEAT STRIP_TAC >> fs[ELIM_CAND_Auxiliary_def,ELIM_CAND_Auxiliary_dec_def]   
 		>> `MEM c (MAP FST p)` by metis_tac [Valid_PileTally_def,FST,MAP] 
                 >> `!d. MEM d h ==> MEM d (MAP FST p)` by metis_tac [Valid_PileTally_def]  
                 >> fs [Valid_Init_CandList_def,NULL,NULL_EQ,
@@ -24,7 +53,7 @@ val Logical_ElimAux_to_Functional = Q.store_thm ("Logical_ElimAux_to_Functional"
 		>> `!(l1:cand list) l2 (c':cand). MEM c' l1 \/ MEM c' l2 ==> MEM c' (l1++l2)`
                      by FULL_SIMP_TAC list_ss [MEM,MEM_APPEND]  
                 >> metis_tac[Logical_list_MEM_VICE_VERCA_TheFunctional,MEM_APPEND,MEM]);    
-   
+         
 
 (* the old proof when bl2 was captured to have more than one cand in it 
                >- (`!c'. MEM c' (h++e) ==> MEM c' l` by metis_tac [MEM,MEM_APPEND]  
@@ -39,11 +68,11 @@ val Logical_ElimAux_to_Functional = Q.store_thm ("Logical_ElimAux_to_Functional"
                      by FULL_SIMP_TAC list_ss [MEM,MEM_APPEND]  
                 >> metis_tac[Logical_list_MEM_VICE_VERCA_TheFunctional,MEM_APPEND,MEM]));    
 *)
-  
+   
 val Functional_ElimAux_to_Logical = Q.store_thm ("Functional_ElimAux_to_Logical",
- `!st qu l c t p np bl2 nbl2 e h nh.
-     ELIM_CAND_Auxiliary_dec c (qu,st,l) t p np bl2 nbl2 e h nh ==> ELIM_CAND_Auxiliary c (qu,st,l) t p np bl2 nbl2 e h nh`,
-           
+ `!st qu l c ba t nt p np bl nbl bl2 e ne h nh.
+     ELIM_CAND_Auxiliary_dec c (qu,st,l) ba t nt p np bl nbl bl2 e ne h nh ==> ELIM_CAND_Auxiliary c (qu,st,l) ba t nt p np bl nbl bl2 e ne h nh`,
+             
     (REPEAT STRIP_TAC  
 	>> rfs[ELIM_CAND_Auxiliary_def,ELIM_CAND_Auxiliary_dec_def]             
          >> fs [NULL,NULL_EQ,Logical_list_MEM_VICE_VERCA_TheFunctional,
@@ -52,20 +81,20 @@ val Functional_ElimAux_to_Logical = Q.store_thm ("Functional_ElimAux_to_Logical"
 	       PileTally_to_PileTally_DEC2,less_than_qu_IMP_LogicalLessThanQuota,
 	       PileTally_to_PileTally_DEC2,bigger_than_cand_LogicallyOK,
 	       MEM,Valid_Init_CandList_def,EQE_REMOVE_ONE_CAND,ALL_DISTINCT_APPEND]
-           >> REPEAT CONJ_TAC) 
+           >> REPEAT CONJ_TAC)   
            >- (`!d'. MEM d' (h++e) ==> MEM d' l` by FULL_SIMP_TAC list_ss [MEM,MEM_APPEND,list_MEM_dec_def,
 	                                             Logical_list_MEM_VICE_VERCA_TheFunctional]   
-             >> metis_tac[MEM_APPEND,MEM]) 	  
-             >- metis_tac [Valid_PileTally_def,PileTally_DEC1_to_PileTally,PileTally_DEC2_IMP_PileTally]
-             >- metis_tac [Valid_PileTally_def,PileTally_DEC1_to_PileTally,PileTally_DEC2_IMP_PileTally]
-             >- metis_tac [Valid_PileTally_def,PileTally_DEC1_to_PileTally,PileTally_DEC2_IMP_PileTally]
+             >> metis_tac[MEM_APPEND,MEM])  	  
+             >- metis_tac [Valid_PileTally_def,PileTally_DEC1_to_PileTally,PileTally_DEC2_IMP_PileTally] 
+             >- metis_tac [Valid_PileTally_def,PileTally_DEC1_to_PileTally,PileTally_DEC2_IMP_PileTally] 
+             >- metis_tac [Valid_PileTally_def,PileTally_DEC1_to_PileTally,PileTally_DEC2_IMP_PileTally] 
              >- (`?L y. l = y::L` by metis_tac[NULL_EQ,list_nchotomy]   
                       >> `MEM y (MAP FST t)` by metis_tac [PileTally_DEC2_IMP_PileTally,MEM] 
                       >> `?l1 q1. t = q1::l1` by metis_tac [MEM_MAP,MEM,list_nchotomy] 
                       >> `!d. MEM d h ==> MEM d l`
                            by metis_tac [MEM_APPEND,Logical_list_MEM_VICE_VERCA_TheFunctional]  
                       >> `!d. MEM d h ==> MEM d (MAP FST t)` by metis_tac [PileTally_DEC2_IMP_PileTally] 
-                    >> metis_tac[PileTally_to_PileTally_DEC2,less_than_qu_IMP_LogicalLessThanQuota])    
+                    >> metis_tac[PileTally_to_PileTally_DEC2,less_than_qu_IMP_LogicalLessThanQuota])     
              >- (`?L y. l = y::L` by metis_tac[NULL_EQ,list_nchotomy]
                      >> `MEM y (MAP FST t)` by metis_tac [PileTally_DEC2_IMP_PileTally,MEM]
                      >> `?l1 q1. t = q1::l1` by metis_tac [MEM_MAP,MEM,list_nchotomy]
@@ -73,7 +102,7 @@ val Functional_ElimAux_to_Logical = Q.store_thm ("Functional_ElimAux_to_Logical"
                          by metis_tac [MEM_APPEND,Logical_list_MEM_VICE_VERCA_TheFunctional]
                      >> `!d. MEM d h ==> MEM d (MAP FST t)` by metis_tac [PileTally_DEC2_IMP_PileTally]
                      >> metis_tac [PileTally_to_PileTally_DEC2,bigger_than_cand_LogicallyOK]));
- 		     
+ 		      
         
 val Logical_TransferAux_to_Functional = Q.store_thm ("Logical_TransferAux_to_Functional",
  `! st qu l ba t t' p np bl bl2 bl2' e e' h h'. TRANSFER_Auxiliary (qu,st,l) ba t t' p np bl bl2 bl2' e e' h h'
@@ -89,7 +118,7 @@ val Logical_TransferAux_to_Functional = Q.store_thm ("Logical_TransferAux_to_Fun
 	    >> fs[PileTally_to_PileTally_DEC1,Valid_PileTally_def,
 	       PileTally_to_PileTally_DEC2,NULL_EQ,NULL,
 	       Valid_Init_CandList_def,LogicalLessThanQu_IMP_less_than_quota,MEM])));
-         
+          
      
 val Functional_TransferAux_to_Logical = Q.store_thm("Functional_TransferAux_to_Logical",
  `! st qu l ba t t' p np bl bl2 bl2' e e' h h'. TRANSFER_Auxiliary_dec (qu,st,l) ba t t' p np bl bl2 bl2' e e' h h'
@@ -111,24 +140,24 @@ val Functional_TransferAux_to_Logical = Q.store_thm("Functional_TransferAux_to_L
                      >> `!d. MEM d h ==> MEM d l`
                          by metis_tac [MEM_APPEND,Logical_list_MEM_VICE_VERCA_TheFunctional]
 		     >> `!d. MEM d h ==> MEM d (MAP FST t)` by metis_tac [PileTally_DEC2_IMP_PileTally]
-                     >> metis_tac[PileTally_to_PileTally_DEC2,less_than_qu_IMP_LogicalLessThanQuota]));  
+                     >> metis_tac[PileTally_to_PileTally_DEC2,less_than_qu_IMP_LogicalLessThanQuota]));   
   
 val Equiv_Functional_Logical_TransferAux = Q.store_thm("Equiv_Functional_Logical_TransferAux",
  `TRANSFER_Auxiliary_dec = TRANSFER_Auxiliary`,
 simp[FUN_EQ_THM,Functional_TransferAux_to_Logical,Logical_TransferAux_to_Functional,FORALL_PROD,EQ_IMP_THM]);
- 
+  
 val Logical_CountAux_to_Functional = Q.store_thm ("Logical_CountAux_to_Functional",
- `! (st: num) (qu: rat) l ba nba t nt p np e h.
-   COUNT_Auxiliary (qu,st,l) ba nba t nt p np e h ==> COUNT_Auxiliary_dec (qu,st,l) ba nba t nt p np e h`,
+ `! (st: num) (qu: rat) l ba nba t nt p np bl nbl e ne h nh.
+   COUNT_Auxiliary (qu,st,l) ba nba t nt p np bl nbl e ne h nh ==> COUNT_Auxiliary_dec (qu,st,l) ba nba t nt p np bl nbl e ne h nh`,
 
       REPEAT STRIP_TAC
        >> fs[COUNT_Auxiliary_def,COUNT_Auxiliary_dec_def] 
           >> metis_tac[Logical_list_MEM_VICE_VERCA_TheFunctional,MEM_APPEND,Valid_PileTally_def,
 	    PileTally_to_PileTally_DEC1,PileTally_to_PileTally_DEC2,Valid_Init_CandList_def,NULL_EQ,NULL]); 
-
+ 
 val Functional_COUNTAux_to_Logical = Q.store_thm("Functional_COUNTAux_to_Logical",
- `! (st: num) (qu: rat) l ba nba t nt p np e h.
-  COUNT_Auxiliary_dec (qu,st,l) ba nba t nt p np e h ==> COUNT_Auxiliary (qu,st,l) ba nba t nt p np e h`,
+ `! (st: num) (qu: rat) l ba nba t nt p np bl nbl e ne h nh.
+  COUNT_Auxiliary_dec (qu,st,l) ba nba t nt p np bl nbl e ne h nh ==> COUNT_Auxiliary (qu,st,l) ba nba t nt p np bl nbl e ne h nh`,
 
   REPEAT STRIP_TAC
    >> fs[COUNT_Auxiliary_dec_def, COUNT_Auxiliary_def]
@@ -136,27 +165,11 @@ val Functional_COUNTAux_to_Logical = Q.store_thm("Functional_COUNTAux_to_Logical
 		  Valid_PileTally_def,PileTally_to_PileTally_DEC1,PileTally_to_PileTally_DEC2,
 	          Valid_Init_CandList_def,NULL_EQ,NULL,Valid_PileTally_def,
 	          PileTally_DEC1_to_PileTally,PileTally_DEC2_IMP_PileTally]);	   		      
-    
-val TAKE_DROP_LENGTH_BACKLOG = Q.store_thm ("TAKE_DROP_LENGTH_BACKLOG",
- `! bl nbl (l1: cand list). nbl = bl ++ l1 ==> (bl = TAKE (LENGTH bl) nbl) /\ (l1 = DROP (LENGTH bl) nbl)`, 
-  
-  REPEAT STRIP_TAC   
-   >- FULL_SIMP_TAC list_ss [TAKE_APPEND1,APPEND_11]    
-   >- (`TAKE (LENGTH bl) nbl = bl` by FULL_SIMP_TAC list_ss [TAKE_APPEND1,TAKE_LENGTH_ID]   
-        >> `nbl = (TAKE (LENGTH bl) nbl) ++ (DROP (LENGTH bl) nbl)` by  FULL_SIMP_TAC list_ss [TAKE_DROP]
-          >> metis_tac[APPEND_11]));  
-
- 
-val DROP_LENGTH = Q.store_thm ("DROP_LENGTH",
- `! bl (l1: cand list). DROP (LENGTH bl) (bl ++ l1) = l1`,
- Induct_on `bl`
-   >- rw[]
-   >- (REPEAT STRIP_TAC 
-     >> FULL_SIMP_TAC list_ss [DROP,MEM]));
      
+
 val Logical_ElectAux_to_Functional = Q.store_thm ("Logical_ElectAux_to_Functional",
- `! st (qu: rat) l ba t p np bl nbl e ne h nh l1. ELECT_Auxiliary (qu,st,l) ba t p np bl nbl e ne h nh l1
-        ==> ELECT_Auxiliary_dec (qu,st,l) ba t p np bl nbl e ne h nh l1`,
+ `! st (qu: rat) l ba t nt p np bl nbl bl2 nbl2 e ne h nh l1. ELECT_Auxiliary (qu,st,l) ba t nt p np bl nbl bl2 nbl2 e ne h nh l1
+        ==> ELECT_Auxiliary_dec (qu,st,l) ba t nt p np bl nbl bl2 nbl2 e ne h nh l1`,
   
    (REPEAT STRIP_TAC
     >> fs[ELECT_Auxiliary_def, ELECT_Auxiliary_dec_def]
@@ -187,11 +200,11 @@ val Logical_ElectAux_to_Functional = Q.store_thm ("Logical_ElectAux_to_Functiona
             >- metis_tac [Valid_PileTally_def,PileTally_to_PileTally_DEC1,PileTally_to_PileTally_DEC2]
             >- metis_tac [Valid_PileTally_def,PileTally_to_PileTally_DEC1,PileTally_to_PileTally_DEC2]
 	    >- metis_tac [Valid_PileTally_def,PileTally_to_PileTally_DEC1,PileTally_to_PileTally_DEC2]);
-        
+         
     
 val Functional_ElectAux_to_Logical = Q.store_thm ("Functional_ElectAux_to_Logical",
- `! st qu l ba t p np bl nbl e ne h nh l1. ELECT_Auxiliary_dec (qu,st,l) ba t p np bl nbl e ne h nh l1 
-                     ==> ELECT_Auxiliary (qu,st,l) ba t p np bl nbl e ne h nh l1`,
+ `! st qu l ba t nt p np bl nbl bl2 nbl2 e ne h nh l1. ELECT_Auxiliary_dec (qu,st,l) ba t nt p np bl nbl bl2 nbl2 e ne h nh l1 
+                     ==> ELECT_Auxiliary (qu,st,l) ba t nt p np bl nbl bl2 nbl2 e ne h nh l1`,
 
  ((REPEAT STRIP_TAC
   >> fs[ELECT_Auxiliary_dec_def,ELECT_Auxiliary_def]
@@ -219,7 +232,7 @@ val Functional_ElectAux_to_Logical = Q.store_thm ("Functional_ElectAux_to_Logica
        >- metis_tac [Valid_PileTally_def,PileTally_DEC1_to_PileTally,PileTally_DEC2_IMP_PileTally]
        >- metis_tac [Logical_list_MEM_VICE_VERCA_TheFunctional]
        >- metis_tac [Logical_list_MEM_VICE_VERCA_TheFunctional])); 
-  
+   
  
 val Logical_TransferExcludedAux_to_Functional = Q.store_thm("Logical_TransferExcludedAux_to_Functional",
  `! qu st l j1 j2. TRANSFER_EXCLUDED_Auxiliary (qu,st,l) j1 j2
@@ -318,6 +331,11 @@ val Functional_TransferExcluded_Aux_to_Logical = Q.store_thm("Functional_Transfe
 	>- rfs[TRANSFER_EXCLUDED_Auxiliary_dec_def])
       >- rfs[TRANSFER_EXCLUDED_Auxiliary_dec_def]));  
            
+val TRANSFER_EXCLUDED_Auxiliary_thm = Q.store_thm("TRANSFER_EXCLUDED_Auxiliary_thm",
+ `TRANSFER_EXCLUDED_Auxiliary_dec = TRANSFER_EXCLUDED_Auxiliary`,
+   simp[FUN_EQ_THM,Logical_TransferExcludedAux_to_Functional,Functional_TransferExcluded_Aux_to_Logical,
+        FORALL_PROD,EQ_IMP_THM]);
+
   
 
  
